named cases in fact "hypothesis"

Wlog.thy
@@ -3,6 +3,36 @@ imports Main
 keywords "wlog" :: "prf_script" and "dummy" :: "prf_script"
 begin
 
+declare[[ML_exception_trace]]
+
+ML Term_Subst.generalize
+ML {* Name.clean_index ("aa__", 0) *}
+
+ML {*
+(* Like Facts.dest_static, but also returns facts that have been overwritten with a new fact of the same name *)
+fun dest_static2 ctx verbose prev_facts facts =
+  let val ctx_generic = Context.Proof ctx
+      fun thms_eq [] [] = true
+        | thms_eq (_::_) [] = false
+        | thms_eq [] (_::_) = false
+        | thms_eq (t::ts) (u::us) = Thm.prop_of t = Thm.prop_of u
+                                    andalso Thm.shyps_of t = Thm.shyps_of u
+                                    andalso Thm.hyps_of t = Thm.hyps_of u
+                                    andalso Thm.tpairs_of t = Thm.tpairs_of u
+                                    (* andalso Thm.get_tags t = Thm.get_tags u *)
+                                    andalso thms_eq ts us
+      fun isprev (name,ths) prev = case Facts.lookup ctx_generic prev name of
+                                      NONE => false
+                                    | SOME (true,ths') => thms_eq ths ths'
+                                    | SOME (false,_) => true (* We don't compare dynamics, we just assume they are not overwritten *)
+  in
+  Facts.fold_static (fn (name, ths) =>
+    if exists (isprev (name, ths)) prev_facts orelse
+      not verbose andalso Facts.is_concealed facts name then I
+    else cons (name, ths)) facts []
+  |> sort_by #1
+  end
+*}
 
 ML {*
 (* Given a theorem thm, replaces all occurrences of the free vars "fixes" by the free vars "fixed".
@@ -17,17 +47,26 @@ fun translate_thm ctx fixes fixed thm =
   let val hyps = Thm.chyps_of thm
       val thm = fold_rev Thm.implies_intr hyps thm
       val idx = Thm.maxidx_of thm + 1
+(* val _ = @{print} (1,thm) *)
       val thm = Thm.generalize ([],map #2 fixes) idx thm
-      val thm = Thm.instantiate ([],map2 (fn (_,n,T) => fn m => (((n,idx),T),Thm.cterm_of ctx (Free(m,T)))) fixes fixed) thm
+(* val _ = @{print} (2,thm,idx,fixes,fixed) *)
+      val thm = Thm.instantiate ([],map2 (fn (_,n,T) => fn m => ((Name.clean_index(n,idx),T),Thm.cterm_of ctx (Free(m,T)))) fixes fixed) thm
+(* val _ = @{print} (3,thm) *)
       val facts = Proof_Context.facts_of ctx
       fun mk_hypnew hyp =
         let val chyp = Thm.cterm_of ctx hyp
             val hyp_thm = Thm.trivial chyp
             val candidates = Facts.could_unify facts hyp
-            fun try_cand cand fallback = hyp_thm OF [cand] handle THM _ => fallback
+            fun try_cand cand fallback = 
+                (* let val hyp = hyp_thm OF [cand]
+                    val hyp_concl = Thm.concl_of hyp
+                    
+                in hyp end *) hyp_thm OF [cand]
+                handle THM _ => fallback
         in fold try_cand candidates hyp_thm end
       val prems = take (length hyps) (Thm.prems_of thm)
       val hypsnew = map mk_hypnew prems
+(* val _ = @{print} (thm,map (Thm.cterm_of ctx) prems) *)
       val thm = thm OF hypsnew
    in thm end
 *}
@@ -54,22 +93,33 @@ fun get_fixes ctx =
 
 ML Assumption.presume_export
 
+lemma x[case_names acase[x y z]]: "a \<Longrightarrow> b \<Longrightarrow> xxx" sorry
+lemma "xxx" apply (cases rule:x) print_cases oops
+ML Rule_Cases.cases_hyp_names
+
 ML {*
 fun wlog (newassm_name,newassm) (fixes:(binding*string*typ) list) (thesis:term) (assms:(string*thm list)list) int state =
   let val _ = @{print} (Proof.goal state)
       val ctx = Proof.context_of state
       val facts = Proof_Context.facts_of ctx
-      val flat_assms = assms |> map snd |> List.concat |> map Thm.prop_of
-      val hyp = Logic.list_implies (newassm :: flat_assms, thesis)
+      (* flat_assms: list of (name,i,t) where t are all assumptions, with i an index to distinguish several propositions in the same fact. (i=0 if there is only one) *)
+      val flat_assms = assms |> map (fn (name,thms) => case thms of [th] => [(name,0,Thm.prop_of th)]
+                                                                  | _ => map_index (fn (i,thm) => (name,i+1,Thm.prop_of thm)) thms) |> List.concat
+      val flat_assms = ("new_assm",0,newassm) :: flat_assms
+      fun idx_name (name,0) = name | idx_name (name,i) = name ^ "_" ^ string_of_int i
+      val _ = List.map (fn (name,i,t) => Output.information ("[Wlog] Assumption " ^ idx_name(name,i) ^ ": " ^ (Syntax.string_of_term ctx t))) flat_assms
+      val hyp = Logic.list_implies (map #3 flat_assms, thesis)
       val hyp = fold (fn (_,a,T) => fn t => Logic.all_const T $ (Term.absfree (a,T) t)) fixes hyp
       val _ = Output.information ("[Wlog] New goal will be: " ^ (Syntax.string_of_term ctx hyp))
-      val state = Proof.presume [] [] [((@{binding hypothesis},[]),[(hyp,[])])] state
+      val case_names = map (fn (name,i,_) => idx_name(name,i)) flat_assms
+      val case_names = Rule_Cases.cases_hyp_names case_names (map (K []) case_names)
+      val state = Proof.presume [] [] [((@{binding hypothesis},[case_names]),[(hyp,[])])] state
 
       fun after_qed (_(*ctx*),_) state = 
       let val let_bindings = Variable.binds_of (Proof.context_of state) |> Vartab.dest
           val state = Proof.next_block state
-          val lost_facts = Facts.dest_static false [Proof_Context.facts_of (Proof.context_of state)] facts
-          val _ = @{print} ("lost_facts",lost_facts)
+          val lost_facts = dest_static2 (Proof.context_of state) false [Proof_Context.facts_of (Proof.context_of state)] facts
+          val _ = @{print} ("lost_facts",map #1 lost_facts)
           val (fixed,state) = Proof.map_context_result (Proof_Context.add_fixes (map (fn (a,_,T) => (a,SOME T,NoSyn)) fixes)) state
           val rename_fixed = ren_frees (map2 (fn (_,a,_) => fn b => (a,b)) fixes fixed)
           val state = fold (fn (name,(_,t)) => Proof.map_context (Variable.bind_term (name,rename_fixed t))) let_bindings state
@@ -133,13 +183,6 @@ lemma
   assumes neq: "a \<noteq> b"
   shows "a+b \<ge> 1"
 proof -
-
-  fix x::int fix x::nat 
-  ML_prf {*
-  val a =   Variable.lookup_fixed @{context} "x" |> Option.valOf
-  val b =  Vartab.lookup (Variable.constraints_of @{context} |> fst) (a,~1)
-  *}
-
   have neq2: "a>b\<or>b>a" using neq bla by auto 
   have comm: "1 \<le> a + b \<Longrightarrow> 1 \<le> b + a" for a b :: nat by auto
 
@@ -148,36 +191,41 @@ proof -
 
   let ?a = a
 
+  have test[]: "\<And>a. b \<noteq> a \<Longrightarrow> a \<noteq> b \<Longrightarrow> 1 \<le> a + b" sorry
+  (* have "1 \<le> a+b" proof (cases rule:test) print_cases case 2  *)
+
+have hyptmp[case_names new_assm neq]: "b \<noteq> a \<Longrightarrow> a \<noteq> b \<Longrightarrow> 1 \<le> a + b" for a sorry
+
+consider "a=a" | "b=b" sorry
+note c = this
+(* have "1 \<le> a + b " proof (cases "True") print_cases case True show ?thesis *)
+
   wlog neq3: "b\<noteq>a" for a shows "a+b\<ge>(1::nat)" assumes neq
-    apply (rule hypothesis)
-    using neq by auto
+  proof (cases rule:hypothesis[where a=a]) print_cases
+    case neq show ?case using assms(2) by blast 
+    case new_assm show ?case using assms(2) by blast 
+  qed
+
+  have aux: "P \<Longrightarrow> (P \<Longrightarrow> Q) \<Longrightarrow> Q" for P Q by metis
 
   ML_prf {* val ctx2 = @{context} *}
-term ?thesis
   wlog geq: "a > b" for a b shows ?thesis assumes neq3
-    apply (cases "a>b")
-     apply (rule hypothesis; simp)
-    apply (subst add.commute)
-     apply (rule hypothesis)
-       using neq apply simp
-      using neq apply simp
-     (* using neq3 apply simp *)
-  by (tactic \<open>ALLGOALS (K all_tac)\<close>)
+  proof (cases "a>b")
+  case True show ?thesis using True hypothesis by blast
+  next case False show ?thesis proof (rule aux, cases rule:hypothesis[of a b])
+    case new_assm show ?case using False neq2 by blast 
+    next case neq3 show ?case using neq2 by auto
+    next assume "1 \<le> b + a" then show "1 \<le> a + b" by linarith 
+    qed
+  qed
 
   note assms = neq neq3
 
-thm neq2 neq
+  have "b<a\<or>a<b" by (simp add: geq)
 
-  ML_prf {*
-    val fixes = [("xxx","a",@{typ nat}),("yyy","b",@{typ nat})]
-    val fixed = ["aa__","ba__"]
-    val neq2' = translate_thm @{context} fixes fixed neq2
-  *}
-  have "b<a\<or>a<b" apply (tactic \<open>resolve_tac @{context} [neq2'] 1\<close>) using assms by auto
+ (* apply (tactic \<open>resolve_tac @{context} [neq2'] 1\<close>) using assms by auto *)
 
-
-
-  wlog tmp: "a=a" for a b shows ?thesis assumes neq geq imports neq2
+  wlog tmp: "a=a" for a b shows ?thesis assumes geq 
     using hypothesis neq geq by metis
 
   from geq have "a \<ge> 1" by auto
